lib/node_rep.v
@@ -2,9 +2,9 @@ From iris.heap_lang Require Import notation.
 
 Local Open Scope Z.
 
-Definition val_rep : Type := val * Z * loc.
+Definition val_rep : Type := Z * Z * loc.
 
-Definition val_v (v: val_rep) : val := v.1.1.
+Definition val_v (v: val_rep) : Z := v.1.1.
 Definition val_ts (v: val_rep) : Z := v.1.2.
 Definition val_next (v: val_rep) : loc := v.2.
 
@@ -13,7 +13,7 @@ Definition valTs : val := λ: "l", Snd (Fst "l").
 Definition valNext : val := λ: "l", Snd "l".
 
 Definition rep_to_val (v: val_rep) : val := 
-  (val_v v, #(val_ts v), #(val_next v)).
+  (#(val_v v), #(val_ts v), #(val_next v)).
 
 Definition node_rep : Type := Z * loc * loc * option loc * val.
 
@@ -43,7 +43,7 @@ Definition dummy_lock : val := #().
 
 
 Lemma fold_rep_to_val (v: val_rep) :
-  ((val_v v, #(val_ts v), #(val_next v)))%V =
+  ((#(val_v v), #(val_ts v), #(val_next v)))%V =
   rep_to_val v.
 Proof. done. Qed.
 
