jellyfish/inv/lazy_inv.v
@@ -1,0 +1,108 @@
+From Coq Require Import Sorting.Sorted.
+
+From iris.base_logic.lib Require Import invariants.
+From iris.algebra Require Import cmra auth frac_auth gmap gset.
+From iris.heap_lang Require Import proofmode.
+
+From SkipList.lib Require Import arg_max.
+From SkipList.jellyfish Require Import code.
+From SkipList.lib Require Import misc node_rep node_lt key_equiv.
+From SkipList.jellyfish Require Import list_equiv.
+
+Class gset_list_unionGS Σ := GsetGS { 
+  gset_nr_A_inGS :> inG Σ (frac_authR (gmapUR Z (arg_maxR Z)));
+  gset_nr_F_inGS :> inG Σ (authR (gsetUR node_rep));
+  gset_Z_disj_inGS :> inG Σ (gset_disjR Z)
+}.
+
+Record sub_gname := mk_sub_gname {
+  s_auth: gname;
+  s_toks: gname
+}.
+
+Record bot_gname := mk_bot_gname {
+  s_frac: gname
+}.
+
+Module LazyListInv (Params: SKIP_LIST_PARAMS).
+  Import Params.
+  Module ListEquiv := ListEquiv Params.
+  Export ListEquiv.
+
+  Section Proofs.
+    Context `{!heapGS Σ, !gset_list_unionGS Σ, !lockG Σ} (lvl: Z).
+
+    Definition from_sub_list (sub: sub_gname) (rep: node_rep) : iProp Σ := 
+      own (s_auth sub) (◯ {[ rep ]})
+      ∗
+      own (s_toks sub) (GSet {[ node_key rep ]}).
+
+    Definition from_bot_list (Smap: gmap Z (prodZ Z)) (rep: node_rep) : iProp Σ := 
+      ∃ (v: val_rep) (vs: gset Z), 
+        (node_val rep) ↦{#1 / 2} rep_to_val v
+        ∗
+        ⌜ Smap !! (node_key rep) = Some (vs, val_ts v) ⌝
+        ∗
+        ⌜ val_v v ∈ vs ⌝.
+
+    Definition node_key_range : gset Z := Zlt_range INT_MIN INT_MAX.
+
+    Definition sub_list_inv (head: node_rep) (Γ: sub_gname) (P: node_rep → iProp Σ) 
+      (S: gset node_rep) (Skeys: gset Z) (L: list node_rep) : iProp Σ := 
+      ⌜ Permutation L (elements S) ⌝
+      ∗
+      ⌜ Sorted node_lt ([head] ++ L ++ [tail]) ⌝
+      ∗
+      ⌜ key_equiv S Skeys ⌝
+      ∗
+      own (s_auth Γ) (● S)
+      ∗
+      own (s_toks Γ) (GSet (node_key_range ∖ Skeys))
+      ∗
+      list_equiv lvl ([head] ++ L) P.
+
+    Definition lazy_list_inv (head: node_rep) (bot: bot_gname)
+      (top_sub: sub_gname) (obot_sub: option sub_gname) : iProp Σ := 
+      ∃ (S: gset node_rep) (Smap: gmap Z (prodZ Z)) (L: list node_rep),
+      match obot_sub with
+      | Some bot_sub => sub_list_inv head top_sub (from_sub_list bot_sub) S (dom Smap) L
+      | None => sub_list_inv head top_sub (from_bot_list Smap) S (dom Smap) L
+                ∗
+                own (s_frac bot) (●F Smap)
+      end.
+
+    Definition levelN (lvl: Z) := nroot .@ "level" .@ lvl.
+
+    Definition is_sub_list (head: node_rep) (bot: bot_gname) (top_sub bot_sub: sub_gname) : iProp Σ := 
+      inv (levelN lvl) (lazy_list_inv head bot top_sub (Some bot_sub)).
+
+    Definition is_bot_list (head: node_rep) (Smap: gmap Z (prodZ Z)) (q: frac)
+      (bot: bot_gname) (sub: sub_gname) : iProp Σ := 
+      own (s_frac bot) (◯F{q} Smap)
+      ∗
+      inv (levelN lvl) (lazy_list_inv head bot sub None).
+
+    
+    Lemma lazy_match_inv (head: node_rep) (bot: bot_gname)
+      (sub: sub_gname) (obot: option sub_gname) :
+      lazy_list_inv head bot sub obot ⊢
+        ∃ (P: node_rep → iProp Σ) (S: gset node_rep) (Skeys: gset Z) (L: list node_rep),
+          sub_list_inv head sub P S Skeys L
+          ∗
+          (sub_list_inv head sub P S Skeys L -∗ lazy_list_inv head bot sub obot).
+    Proof.
+      destruct obot as [bot_sub|].
+      + iIntros "Hsub"; unfold lazy_list_inv.
+        iDestruct "Hsub" as (S Smap L) "Hsub".
+        iExists (from_sub_list bot_sub), S, (dom Smap), L.
+        iFrame. iIntros "Hsub".
+        iExists S, Smap, L; iFrame.
+      + iIntros "Hbot"; unfold lazy_list_inv.
+        iDestruct "Hbot" as (S Smap L) "(Hsub & Hown)".
+        iExists (from_bot_list Smap), S, (dom Smap), L.
+        iFrame. iIntros "Hsub".
+        iExists S, Smap, L; iFrame.
+    Qed.
+
+  End Proofs.
+End LazyListInv.
