jellyfish/inv/list_equiv.v
@@ -1,0 +1,318 @@
+From Coq Require Import Sorting.Sorted.
+
+From iris.base_logic.lib Require Import invariants.
+From iris.heap_lang Require Import proofmode.
+
+From SkipList.jellyfish Require Import code.
+From SkipList.lib Require Import misc node_rep node_lt key_equiv.
+
+
+Local Open Scope Z.
+
+Module ListEquiv (Params: SKIP_LIST_PARAMS).
+  Import Params.
+  Module SkipList := SkipList Params.
+  Export SkipList.
+
+  Section Proofs.
+    Context `{!heapGS Σ, !lockG Σ} (lvl: Z).
+
+    Definition is_array (next: loc) (h: Z) : iProp Σ := 
+      ∃ (vs: list val), next ↦∗{#1 / 2} vs ∗ ⌜ length vs = Z.to_nat h ⌝.
+
+    Fixpoint list_equiv (L: list node_rep) (P: node_rep → iProp Σ) : iProp Σ :=
+      match L with
+      | nil => True
+      | pred :: succs => 
+        match succs with
+        | nil => ∃ (γ: gname) (h: Z) (t: loc), 
+                 (node_next pred +ₗ lvl) ↦{#1 / 2} #t
+                 ∗
+                 t ↦□ rep_to_node tail
+                 ∗
+                 is_lock γ (node_lock pred) (is_array (node_next pred) h)
+                 ∗
+                 ⌜ lvl < h ⌝
+
+        | succ :: _ => ∃ (γ: gname) (h: Z) (s: loc), 
+                       (node_next pred +ₗ lvl) ↦{#1 / 2} #s
+                       ∗
+                       s ↦□ rep_to_node succ
+                       ∗
+                       is_lock γ (node_lock pred) (is_array (node_next pred) h)
+                       ∗
+                       ⌜ lvl < h ⌝
+                       ∗
+                       P succ
+                       ∗
+                       list_equiv succs P
+        end
+      end. 
+    
+
+    Lemma list_equiv_cons (rep: node_rep) (L: list node_rep)
+      (P: node_rep → iProp Σ) :
+      list_equiv (rep :: L) P ⊢ 
+        (list_equiv L P ∗ (list_equiv L P -∗ list_equiv (rep :: L) P)).
+    Proof.
+      destruct L as [|n].
+      + iIntros "Hrep". by iFrame.
+      + iIntros "Hlist". 
+        iDestruct "Hlist" as (γ h s) "(Hpt & Hs & Hlock & Hh & HP & Hmatch)".
+        iFrame. iIntros "Hlist". iFrame.
+        iExists γ, h, s. iFrame.
+    Qed.
+
+    Lemma list_equiv_split (pred succ: node_rep) (L L1 L2: list node_rep) 
+      (P: node_rep → iProp Σ) :
+      L ++ [tail] = L1 ++ [pred; succ] ++ L2 →
+      list_equiv L P ⊢ 
+        ∃ (s: loc),
+          (node_next pred +ₗ lvl) ↦{#1 / 2} #s
+          ∗
+          s ↦□ rep_to_node succ
+          ∗
+          ((node_next pred +ₗ lvl) ↦{#1 / 2} #s -∗ list_equiv L P).
+    Proof.
+      revert L. induction L1 => L HL.
+      + destruct L as [|curr L].
+        { exfalso. inversion HL. }
+        inversion HL as [[H0 HL']]; subst.
+        destruct L as [|curr L].
+        - inversion HL'; subst.
+          iIntros "Hlist".
+          iDestruct "Hlist" as (γ h t) "(Hpt & #Ht & #Hlock & Hh)".
+          iExists t. iFrame "# ∗".
+          iIntros "Hpt". 
+          iExists γ, h, t. iFrame "# ∗".
+        - inversion HL'; subst.
+          iIntros "Hlist". 
+          iDestruct "Hlist" as (γ h s) "(Hpt & #Hs & #Hlock & Hh & Hmatch)".
+          iExists s. iFrame "# ∗".
+          iIntros "Hpt". 
+          iExists γ, h, s. iFrame "# ∗".
+      + destruct L as [|curr L].
+        { 
+          exfalso. inversion HL  as [[H0 HL']]; subst. 
+          destruct L1; inversion HL'.
+        }
+        inversion HL as [[H0 HL']]; subst.
+
+        destruct L as [|curr L].
+        { 
+          exfalso. 
+          destruct L1; inversion HL. 
+          destruct L1; inversion HL.
+        }
+        
+        iIntros "Hlist".
+        iPoseProof (list_equiv_cons with "Hlist") as "(Hlist & Himp)".
+        iPoseProof (IHL1 with "Hlist") as "Hlist"; auto.
+        iDestruct "Hlist" as (s) "(Hpt & #Hs & Himp')".
+        iExists s. iFrame "# ∗".
+        iIntros "Hpt".
+        iApply "Himp". iApply "Himp'". iFrame.
+    Qed.
+
+    Lemma list_equiv_invert_L (L: list node_rep) (head pred: node_rep) 
+      (P: node_rep → iProp Σ) :
+      In pred L →
+      list_equiv ([head] ++ L) P ⊢ 
+        ∃ (γ: gname) (h: Z) (s: loc) (succ: node_rep), 
+          (⌜ In succ L ⌝ ∨ ⌜ succ = tail ⌝)
+          ∗
+          (node_next pred +ₗ lvl) ↦{#1/2} #s
+          ∗
+          s ↦□ rep_to_node succ
+          ∗ 
+          is_lock γ (node_lock pred) (is_array (node_next pred) h)
+          ∗
+          ⌜ lvl < h ⌝
+          ∗
+          P pred
+          ∗
+          ((node_next pred +ₗ lvl) ↦{#1/2} #s 
+            ∗ 
+            P pred 
+            -∗ 
+              list_equiv ([head] ++ L) P).
+    Proof.
+      iIntros (Hin) "Hlist".
+      iRevert (head Hin) "Hlist".
+      iInduction L as [|succ L] "IHL"; iIntros (head) "Hin"; first by iExFalso.
+      iDestruct "Hin" as "[%Heq|Hin]"; subst; iIntros "Hlist".
+      + iDestruct "Hlist" as (γ h s) "(Hpt & #Hs & #Hlock & Hh & HP & Hlist)".
+        destruct L as [|next L]; subst.
+        - iDestruct "Hlist" as (γ' h' t) "(Hpt' & #Ht & #Hlock' & #Hh')".
+          iExists γ', h', t, tail. iFrame "# ∗".
+          iSplit; first by iRight.
+          iIntros "(Hpt' & HP)". 
+          iExists γ, h, s. iFrame "# ∗".
+          iExists γ', h', t. iFrame "# ∗".
+        - iDestruct "Hlist" as (γ' h' n) "(Hpt' & #Hn & #Hlock' & #Hh' & Hmatch)".
+          iExists γ', h', n, next. iFrame "# ∗".
+          iSplit; first by iLeft; iRight; iLeft.
+          iIntros "(Hpt' & HP)". 
+          iExists γ, h, s. iFrame "# ∗".
+          iExists γ', h', n. iFrame "# ∗".
+      + iPoseProof (list_equiv_cons with "Hlist") as "(Hlist & Himp)".
+        iPoseProof ("IHL" with "Hin") as "Himp'".
+        iPoseProof ("Himp'" with "Hlist") as "Hlist".
+        iDestruct "Hlist" as (γ h n next) "(%Hnext & Hpt & #Hn & #Hlock & #Hh & HP & Himp')".
+        iExists γ, h, n, next. iFrame "# ∗".
+        iSplit.
+        { iPureIntro; destruct Hnext; first left; by right. }
+        iIntros "(Hpt & HP)". 
+        iApply "Himp". iApply "Himp'". iFrame.
+    Qed.
+
+    Lemma list_equiv_invert (L: list node_rep) (head pred: node_rep) 
+      (P: node_rep → iProp Σ) :
+      pred = head ∨ In pred L →
+      list_equiv ([head] ++ L) P ⊢ 
+        ∃ (γ: gname) (h: Z) (s: loc) (succ: node_rep),
+          (⌜ In succ L ⌝ ∨ ⌜ succ = tail ⌝)
+          ∗
+          (node_next pred +ₗ lvl) ↦{#1/2} #s
+          ∗
+          s ↦□ rep_to_node succ
+          ∗ 
+          is_lock γ (node_lock pred) (is_array (node_next pred) h)
+          ∗
+          ⌜ lvl < h ⌝
+          ∗
+          ((node_next pred +ₗ lvl) ↦{#1/2} #s -∗ list_equiv ([head] ++ L) P).
+    Proof.
+      intros Hin; destruct Hin as [Heq|Hin]; first subst.
+      + iIntros "Hlist". destruct L as [|next L].
+        - iDestruct "Hlist" as (γ h t) "(Hpt & #Ht & #Hlock & #Hh)".
+          iExists γ, h, t, tail. iFrame "# ∗".
+          iSplit; first by iRight.
+          iIntros "Hpt". 
+          iExists γ, h, t. iFrame "# ∗".
+        - iDestruct "Hlist" as (γ h n) "(Hpt & #Hn & #Hlock & #Hh & ?)".
+          iExists γ, h, n, next. iFrame "# ∗".
+          iSplit; first by repeat iLeft.
+          iIntros "Hpt". 
+          iExists γ, h, n. iFrame "# ∗".
+      + iIntros "Hlist".
+        iPoseProof (list_equiv_invert_L with "Hlist") as "Hlist"; first done.
+        iDestruct "Hlist" as (γ h s succ) "(? & ? & ? & ? & ? & ? & Himp)".
+        iExists γ, h, s, succ. iFrame.
+        iIntros "?". iApply "Himp". iFrame.
+    Qed.
+
+    Lemma list_equiv_insert (s n: loc) (head pred new succ: node_rep) 
+      (L: list node_rep) (γ': gname) (h': Z) (P: node_rep → iProp Σ) :
+      node_key new < node_key tail →
+      node_key pred < node_key new < node_key succ →
+      Sorted node_lt ([head] ++ L ++ [tail]) →
+      pred = head ∨ In pred L →
+      list_equiv ([head] ++ L) P ⊢ 
+        s ↦□ rep_to_node succ
+        ∗ 
+        (node_next pred +ₗ lvl) ↦{#1/2} #s
+        ∗ 
+        (node_next new +ₗ lvl) ↦{#1/2} #s
+        ∗
+        n ↦□ rep_to_node new
+        ∗ 
+        is_lock γ' (node_lock new) (is_array (node_next new) h')
+        ∗
+        ⌜ lvl < h' ⌝
+        ∗
+        P new
+        -∗ 
+          ∃ (L' L1 L2: list node_rep), 
+            (node_next pred +ₗ lvl) ↦ #s
+            ∗
+            ⌜ [head] ++ L ++ [tail] = L1 ++ [pred; succ] ++ L2 ⌝
+            ∗
+            ⌜ Sorted node_lt ([head] ++ L' ++ [tail]) ⌝
+            ∗
+            ⌜ Permutation ([head] ++ L') ([head; new] ++ L) ⌝ 
+            ∗
+            ((node_next pred +ₗ lvl) ↦{#1/2} #n -∗ list_equiv ([head] ++ L') P).
+    Proof.
+      iIntros (Hnew Hrange Hsort Hin) .
+      iIntros "Hlist (Hs & Hpt & Hpt' & Hn & Hlock' & Hh' & HP')".
+      remember ([head] ++ L) as L' eqn:HeqL'.
+      rewrite -in_inv in Hin.
+
+      iRevert (head L HeqL' Hsort Hin) "Hlist Hs Hpt Hpt' Hn Hlock' Hh' HP'".
+      iInduction L' as [|pred'] "IHL'".
+      { iIntros (head L Hfalse); inversion Hfalse. }
+
+      iIntros (head L HeqL' Hsort).
+      inversion HeqL'; subst.
+      iIntros (Hin); inversion Hin as [Heq|HinL].
+      + subst.
+        iIntros "Hlist #Hs Hpt Hpt' #Hn #Hlock' Hh' HP'".
+        destruct L as [|succ' L].
+        - iDestruct "Hlist" as (γ h t) "(Hpt'' & #Ht & #Hlock & Hh)".
+          iDestruct (mapsto_agree with "Hpt Hpt''") as %Heq.
+          assert (s = t) as -> by congruence.
+          iDestruct (mapsto_agree with "Hs Ht") as %->%rep_to_node_inj.
+          
+          iExists (new :: nil), nil, nil.
+          iFrame. iSplit; first done. iSplit.
+          { 
+            iPureIntro; apply Sorted_cons; econstructor; auto.
+            all: unfold node_lt; lia.
+          }
+          iSplit; first auto.
+          iIntros "Hpt". 
+          iExists γ, h, n. iFrame "# ∗".
+          iExists γ', h', t. iFrame "# ∗".
+        - iDestruct "Hlist" as (γ h s') "(Hpt'' & #Hs' & #Hlock & Hh & Hmatch)".
+          iDestruct (mapsto_agree with "Hpt Hpt''") as %Heq.
+          assert (s = s') as <- by congruence.
+          iDestruct (mapsto_agree with "Hs Hs'") as %<-%rep_to_node_inj.
+
+          iExists (new :: succ :: L), nil, (L ++ [tail]).
+          iFrame. iSplit; first done. iSplit.
+          { 
+            iPureIntro.
+            repeat apply Sorted_inv in Hsort as (Hsort&?).
+            repeat econstructor; auto. 
+            all: unfold node_lt; lia.
+          }
+          iSplit; first auto.
+          iIntros "Hpt". 
+          iExists γ, h, n. iFrame "# ∗".
+          iExists γ', h', s. iFrame "# ∗".
+      + destruct L as [|next L]; first by inversion HinL.
+        iIntros "Hlist #Hs Hpt Hpt' #Hn #Hlock' Hh' HP'".
+
+        simpl in Hsort; apply Sorted_inv in Hsort as (Hsort&Hhd).
+        iDestruct "Hlist" as (γ h x) "(Hpt'' & #Hx & Hlock & Hh & HP & Hmatch)".
+        iPoseProof ("IHL'" $! next L with "[%] [%] [%] [$] [$] [$] [$] [$] [$] [$] [$]") 
+          as "Hclose"; auto.
+        
+        iDestruct "Hclose" as (L' L1 L2) "(Hpt' & %Hsplit & %Hsort' & %Hperm' & Himp')".
+        iExists (next :: L'), (head :: L1), L2. iFrame.
+        iSplit.
+        {
+          rewrite /= in Hsplit.
+          rewrite /= Hsplit //.
+        }
+        iSplit.
+        {
+          iPureIntro. inversion Hhd.
+          apply Sorted_inv in Hsort' as (Hsort'&?).
+          repeat econstructor; auto.
+        }
+        iSplit.
+        {
+          iPureIntro. 
+          simpl in Hperm'; rewrite Hperm'. 
+          econstructor; econstructor.
+        }
+
+        iIntros "Hpt". iExists γ, h, x.
+        iPoseProof ("Himp'" with "Hpt") as "Hlist".
+        iFrame "# ∗".
+    Qed.
+
+  End Proofs.
+End ListEquiv.
