jellyfish/inv/skip_inv.v
@@ -1,0 +1,174 @@
+From iris.base_logic.lib Require Import invariants.
+From iris.heap_lang Require Import proofmode.
+
+From SkipList.lib Require Import arg_max.
+From SkipList.jellyfish Require Import code.
+From SkipList.lib Require Import misc node_rep node_lt key_equiv.
+From SkipList.jellyfish.inv Require Import list_equiv lazy_inv.
+
+
+Local Open Scope Z.
+
+Module SkipListInv (Params: SKIP_LIST_PARAMS).
+  Import Params.
+  Module Invariant := LazyListInv Params.
+  Export Invariant.
+
+  Section Proofs.
+    Context `{!heapGS Σ, !gset_list_unionGS Σ, !lockG Σ}.
+
+    Fixpoint skip_list_equiv (lvl: Z) (head: node_rep) (Smap: gmap Z (prodZ Z)) 
+      (q: frac) (bot: bot_gname) (subs: list sub_gname) : iProp Σ :=
+      match subs with
+      | nil => False
+      | top_sub :: bot_subs =>
+        match bot_subs with
+        | nil =>
+          ⌜ lvl = 0 ⌝
+          ∗
+          is_bot_list lvl head Smap q bot top_sub
+
+        | bot_sub :: _ =>
+          ⌜ lvl > 0 ⌝
+          ∗
+          is_sub_list lvl head bot top_sub bot_sub
+          ∗
+          skip_list_equiv (lvl - 1) head Smap q bot bot_subs
+        end
+      end.
+
+    Definition is_skip_list (v: val) (Smap: gmap Z (prodZ Z)) (q: frac) 
+      (bot: bot_gname) (subs: list sub_gname) : iProp Σ := 
+      ∃ (l:loc) (head: node_rep),
+      ⌜ #l = v ⌝
+      ∗
+      l ↦{#q} rep_to_node head
+      ∗
+      ⌜ node_key head = INT_MIN ⌝
+      ∗
+      skip_list_equiv MAX_HEIGHT head Smap q bot subs.
+
+    
+    Lemma skip_list_equiv_cons (head: node_rep) (lvl: Z) (Smap: gmap Z (prodZ Z)) 
+      (q: frac) (bot: bot_gname) (top_sub: sub_gname) (bot_subs: list sub_gname) :
+      skip_list_equiv lvl head Smap q bot (top_sub :: bot_subs) ⊢ 
+        ∃ (obot: option sub_gname),
+          inv (levelN lvl) (lazy_list_inv lvl head bot top_sub obot)
+          ∗
+          skip_list_equiv lvl head Smap q bot (top_sub :: bot_subs).
+    Proof.
+      destruct bot_subs as [|bot_sub bot_subs].
+      + iIntros "Htop". iExists None.
+        iDestruct "Htop" as "(? & ? & #Hinv)".
+        iFrame "# ∗".
+      + iIntros "Hlist". iExists (Some bot_sub).
+        iDestruct "Hlist" as "(? & #Hinv & ?)".
+        iFrame "# ∗".
+    Qed.
+
+    Lemma skip_list_equiv_inv (lvl: Z) (head: node_rep) (Smap: gmap Z (prodZ Z)) 
+      (q: frac) (bot: bot_gname) (subs: list sub_gname) :
+      skip_list_equiv lvl head Smap q bot subs ⊢
+        ∃ (sub: sub_gname),
+        ⌜ last subs = Some sub ⌝
+        ∗
+        is_bot_list 0 head Smap q bot sub
+        ∗
+        (is_bot_list 0 head Smap q bot sub -∗ skip_list_equiv lvl head Smap q bot subs).
+    Proof.
+      iRevert (lvl).
+      iInduction subs as [|top_sub subs] "IHsubs";
+        iIntros (lvl) "Hlist"; 
+        first by iExFalso.
+      
+      destruct subs as [|bot_sub subs].
+      + iDestruct "Hlist" as "(%Hlvl & Hbot)".
+        rewrite Hlvl.
+        iExists top_sub; iFrame.
+        iSplit; first done.
+        iIntros "Hbot"; by iFrame.
+      + iDestruct "Hlist" as "(Hlvl & Hsub & Hmatch)".
+        iPoseProof ("IHsubs" with "Hmatch") as "Hlist".
+        iDestruct "Hlist" as (sub) "(Hlast & Hbot & Himp)".
+        iExists sub; iFrame.
+        iIntros "Hbot".
+        iPoseProof ("Himp" with "Hbot") as "Hlist".
+        iFrame.
+    Qed.
+
+    Lemma skip_list_equiv_sep (lvl: Z) (head: node_rep) (Smap: gmap Z (prodZ Z)) 
+      (q1 q2: frac) (bot: bot_gname) (subs: list sub_gname) :
+      skip_list_equiv lvl head Smap (q1 + q2) bot subs ⊢ 
+        skip_list_equiv lvl head Smap q1 bot subs ∗ skip_list_equiv lvl head Smap q2 bot subs.
+    Proof.
+      iRevert (lvl head).
+      iInduction subs as [|top_sub bot_subs] "IHsubs"; 
+        iIntros (lvl head) "Hlist"; 
+        first by iExFalso.
+
+      destruct bot_subs as [|bot_sub bot_subs].
+      + iDestruct "Hlist" as "(%Hlvl & Hown_frag & #Hinv)".
+        iDestruct "Hown_frag" as "(Hown_frag1 & Hown_frag2)".
+        by iFrame "# ∗".
+      + iDestruct "Hlist" as "(%Hlvl & #Hinv & Hmatch)".
+        iPoseProof ("IHsubs" with "Hmatch") as "(Hlist1 & Hlist2)".
+        iSplitL "Hlist1"; by iFrame "# ∗".
+    Qed.
+
+    Lemma skip_list_equiv_join (lvl: Z) (head: node_rep) (Smap1 Smap2: gmap Z (prodZ Z)) 
+      (q1 q2: frac) (bot: bot_gname) (subs: list sub_gname) :
+      skip_list_equiv lvl head Smap1 q1 bot subs ∗ skip_list_equiv lvl head Smap2 q2 bot subs ⊢ 
+        skip_list_equiv lvl head (merge op Smap1 Smap2) (q1 + q2) bot subs.
+    Proof.
+      iRevert (lvl head).
+      iInduction subs as [|top_sub bot_subs] "IHsubs"; 
+        iIntros (lvl head) "(Hlist1 & Hlist2)"; 
+        first by iExFalso.
+
+      destruct bot_subs as [|bot_sub bot_subs].
+      + iDestruct "Hlist1" as "(%Hlvl & Hown_frag1 & #Hinv)".
+        iDestruct "Hlist2" as "(_ & Hown_frag2 & _)".
+        iCombine "Hown_frag1 Hown_frag2" as "Hown_frag".
+        by iFrame "# ∗".
+      + iDestruct "Hlist1" as "(%Hlvl & #Hinv & Hmatch1)".
+        iDestruct "Hlist2" as "(_ & _ & Hmatch2)".
+        iCombine "Hmatch1 Hmatch2" as "Hmatch".
+        iPoseProof ("IHsubs" with "Hmatch") as "Hlist".
+        by iFrame "# ∗".
+    Qed.
+      
+    Lemma is_skip_list_sep (v: val) (Smap: gmap Z (prodZ Z)) 
+      (q1 q2: frac) (bot: bot_gname) (subs: list sub_gname) :
+      is_skip_list v Smap (q1 + q2) bot subs ⊢ 
+        is_skip_list v Smap q1 bot subs ∗ is_skip_list v Smap q2 bot subs.
+    Proof.
+      iIntros "Hlist".
+      iDestruct "Hlist" as (h head) "(%Hv & Hpt & %Hmin & Hlist)".
+
+      iDestruct "Hpt" as "(Hpt1 & Hpt2)".
+      iDestruct (skip_list_equiv_sep with "Hlist") as "(Hlist1 & Hlist2)".
+
+      iSplitL "Hpt1 Hlist1"; iExists h, head; by iFrame.
+    Qed.      
+    
+    Lemma is_skip_list_join (v: val) (Smap1 Smap2: gmap Z (prodZ Z))
+      (q1 q2: frac) (bot: bot_gname) (subs: list sub_gname) :
+      is_skip_list v Smap1 q1 bot subs ∗ is_skip_list v Smap2 q2 bot subs ⊢ 
+        is_skip_list v (merge op Smap1 Smap2) (q1 + q2) bot subs.
+    Proof.
+      iIntros "(Hlist1 & Hlist2)".
+      iDestruct "Hlist1" as (h head) "(%Hv & Hpt1 & %Hmin & Hlist1)".
+      iDestruct "Hlist2" as (h' head') "(%Hv' & Hpt2 & _ & Hlist2)".
+
+      assert (h = h') as <- by congruence.
+      iDestruct (mapsto_agree with "Hpt1 Hpt2") as %<-%rep_to_node_inj.
+      iCombine "Hpt1 Hpt2" as "Hpt".
+
+      iCombine "Hlist1 Hlist2" as "Hlist".
+      rewrite skip_list_equiv_join.
+
+      iExists h, head. by iFrame.
+    Qed.
+
+  End Proofs.
+End SkipListInv.
