jellyfish/spec/get.v
@@ -1,0 +1,194 @@
+From iris.algebra Require Import auth frac_auth gmap gset.
+From iris.heap_lang Require Import proofmode.
+
+From SkipList.lib Require Import arg_max.
+From SkipList.jellyfish Require Import code.
+From SkipList.lib Require Import misc node_rep node_lt key_equiv.
+From SkipList.jellyfish.inv Require Import list_equiv lazy_inv skip_inv.
+From SkipList.jellyfish.spec Require Import find.
+
+
+Local Open Scope Z.
+
+Module GetSpec (Params: SKIP_LIST_PARAMS).
+  Import Params.
+  Module Find := FindSpec Params.
+  Export Find.
+
+  Section Proofs.
+    Context `{!heapGS Σ, !gset_list_unionGS Σ, !lockG Σ}.
+    
+    Theorem findPred_spec (key lvl: Z) (head curr: node_rep) 
+      (Smap: gmap Z (prodZ Z)) (bot: bot_gname) 
+      (top_sub: sub_gname) (bot_subs: list sub_gname) :
+      {{{ 
+        skip_list_equiv lvl head Smap 1 bot (top_sub :: bot_subs)
+        ∗
+        (⌜ curr = head ⌝ ∨ own (s_auth top_sub) (◯ {[ curr ]}))
+        ∗
+        ⌜ node_key curr < key < INT_MAX ⌝
+      }}}
+        findPred (rep_to_node curr) #key #lvl
+      {{{ pred succ sub, RET ((rep_to_node pred), (rep_to_node succ));
+        skip_list_equiv lvl head Smap 1 bot (top_sub :: bot_subs)
+        ∗
+        ⌜ last (top_sub :: bot_subs) = Some sub ⌝
+        ∗
+        (own (s_auth sub) (◯ {[ succ ]}) ∨ ⌜ succ = tail ⌝)
+        ∗
+        ⌜ key ∈ dom Smap ↔ node_key succ = key ⌝
+      }}}.
+    Proof.
+      iIntros (Φ) "(Hlist & Hown_curr & Hrange) HΦ".
+      iRevert (curr head lvl top_sub bot_subs) "Hlist Hown_curr Hrange HΦ".
+      iLöb as "IH".
+      iIntros (curr head lvl top_sub bot_subs) "Hlist #Hown_curr %Hrange HΦ".
+
+      wp_lam. wp_let. wp_let.
+      destruct bot_subs as [|bot_sub].
+      + iDestruct "Hlist" as "(%Hlvl & (Hown_frag & #Hinv))".
+        wp_apply (find_bot_spec with "[Hown_frag]").
+        { by iFrame "# ∗". }
+        iIntros (pred succ) "(Hown_frag & %Hpred_key & #Hown_succ & %Hkey_in_S)".
+
+        wp_pures. case_bool_decide; wp_if.
+        - iModIntro. iApply "HΦ". 
+          by iFrame "# ∗".
+        - exfalso; congruence.
+      + iDestruct "Hlist" as "(%Hlvl & #Hinv & Hmatch)".
+        unfold is_sub_list.
+        wp_apply find_sub_spec.
+        { by iFrame "# ∗". }
+        iIntros (pred succ) "(%Hrange' & #Hown_pred & #Hown_succ & _)".
+
+        wp_pures. case_bool_decide as Hcase; wp_if.
+        - exfalso; inversion Hcase; lia.
+        - wp_bind (Fst _).
+          iInv (levelN lvl) as (S Smap' L) "Hsub" "Hclose".
+          iDestruct "Hsub" as "(>%Hperm & >%Hsort & >%Hequiv & >Hown_auth & >Hown_toks & Hlist)".
+
+          iDestruct "Hown_pred" as "[%Heq | #Hown_pred]".
+          * wp_proj.            
+            iMod ("Hclose" with "[Hlist Hown_auth Hown_toks]") as "_".
+            { iNext; iExists S, Smap', L; by iFrame. }
+
+            iModIntro; wp_pures.
+            iApply ("IH" with "[$] [] [%]").
+            { by iLeft. }
+            { lia. }
+            iNext; iIntros (? ? ?) "(? & ? & ? & ?)".
+            iApply "HΦ". by iFrame "# ∗".
+          * iAssert ⌜ In pred L ⌝%I with "[Hown_auth]" as %Hin.
+            {
+              iDestruct (own_valid_2 with "Hown_auth Hown_pred") 
+                as %[Hvalid%gset_included]%auth_both_valid_discrete.
+              rewrite -elem_of_list_In Hperm elem_of_elements.
+              iPureIntro; set_solver.
+            }
+
+            rewrite list_equiv_invert_L; last done.
+            iDestruct "Hlist" as (γ h s' succ') "(>%Hsucc'_range & Hpt' & #Hs' & Hlock & #Hlvl & HP & Himp)".
+            iDestruct "HP" as"(>Hauth_pred & >Htoks_pred)".
+
+            assert ({[ pred ]} = {[ pred ]} ⋅ {[ pred ]}) as -> by set_solver.
+            iDestruct "Hauth_pred" as "(Hauth_pred & ?)".
+            assert ({[ pred ]} = {[ pred ]} ⋅ {[ pred ]}) as <- by set_solver.
+
+            wp_proj.
+            iPoseProof ("Himp" with "[$]") as "Hlist".
+            iMod ("Hclose" with "[Hlist Hown_auth Hown_toks]") as "_".
+            { iNext; iExists S, Smap', L; by iFrame. }
+
+            iModIntro; wp_pures.
+            iApply ("IH" with "[$] [Hauth_pred] [%]").
+            { by iRight. }
+            { lia. }
+            iNext; iIntros (? ? ?) "(? & ? & ? & ?)".
+            iApply "HΦ". by iFrame "# ∗".
+    Qed.
+    
+    Theorem get_spec (v: val) (key: Z) (Smap: gmap Z (prodZ Z)) 
+      (bot: bot_gname) (subs: list sub_gname)
+      (Hrange: INT_MIN < key < INT_MAX) :
+      {{{ is_skip_list v Smap 1 bot subs }}}
+        get v #key
+      {{{ (opt: val), RET opt;
+        is_skip_list v Smap 1 bot subs
+        ∗
+        (( ⌜ opt = NONEV ⌝ ∗ ⌜ Smap !! key = None ⌝ )
+        ∨
+        (∃ (res ts: Z) (pair: prodZ Z), 
+            ⌜ opt = SOMEV (#res, #ts) ⌝ ∗ ⌜ Smap !! key = Some pair ⌝
+            ∗
+            ⌜ res ∈ fst pair ⌝ ∗ ⌜ ts = snd pair ⌝ ))
+      }}}.
+    Proof.
+      iIntros (Φ) "H HΦ".
+      iDestruct "H" as (h head) "(%Hv & Hpt & %Hmin & Hlist)".
+      wp_lam. wp_let. rewrite -Hv. wp_load. wp_let.
+      destruct subs as [|sub subs]; first by iExFalso.
+
+      wp_apply (findPred_spec with "[Hlist]").
+      { iFrame. iSplit. by iLeft. iPureIntro; lia. }
+
+      iIntros (pred succ bot_sub) "(Hlist & %Hlast & #Hown & %Hkey_in_dom)".
+      wp_pures. wp_lam. wp_pures.
+      
+      case_bool_decide as Hcase; wp_if.
+      + wp_lam. wp_pures.
+        rewrite skip_list_equiv_inv.
+        iDestruct "Hlist" as (bot_sub') "(%Hlast' & (Hown_frag & #Hinv) & Himp)".
+        assert (bot_sub = bot_sub') as <- by congruence.
+
+        wp_bind (Load _).
+        iInv (levelN 0) as (S ? L) "(Hinv_sub & >Hown_frac)" "Hclose".
+        iDestruct "Hinv_sub" as "(>%Hperm & >%Hsort & >%Hequiv & >Hown_auth & >Hown_toks & Hlist)".
+        iDestruct (own_valid_2 with "Hown_frac Hown_frag") 
+          as %->%frac_auth_agree_L.
+
+        iAssert ⌜ In succ L ⌝%I with "[Hown_auth]" as %Hsucc.
+        {
+          iDestruct "Hown" as "[Hown|%Hfalse]"; last first.
+          {
+            assert (key = node_key tail) as -> by congruence.
+            rewrite /tail/node_key/= in Hrange; lia.
+          }
+
+          iDestruct (own_valid_2 with "Hown_auth Hown") 
+            as %[Hvalid%gset_included]%auth_both_valid_discrete.
+          rewrite -elem_of_list_In Hperm elem_of_elements.
+          iPureIntro; set_solver.
+        }
+
+        rewrite (list_equiv_invert_L 0 L head succ); last done.
+        iDestruct "Hlist" as (γ' h' s' succ') "(_ & Hpt' & _ & _ & _ & HP & Himp')".
+        iDestruct "HP" as (val vs) "(Hval & >%Hsome & >%Hin)".
+
+        wp_load.
+        iPoseProof ("Himp'" with "[Hpt' Hval]") as "Hlist".
+        { iFrame; iExists val, vs; by iFrame. }
+        iMod ("Hclose" with "[Hlist Hown_auth Hown_toks Hown_frac]") as "_".
+        { iNext; iExists S, Smap, L; by iFrame. }
+        iPoseProof ("Himp" with "[$]") as "Hlist".
+
+        iModIntro. wp_pures.
+        iModIntro; iApply "HΦ". 
+        iSplit.
+        { iExists h, head; by iFrame. }
+
+        iPureIntro; right.
+        exists (val_v val), (val_ts val), (vs, val_ts val).
+        inversion Hcase; subst.
+        rewrite //.
+      + iModIntro; iApply "HΦ". 
+        iSplit. 
+        { iExists h, head; by iFrame. }
+        
+        iPureIntro; left.
+        split; first done.
+        rewrite -not_elem_of_dom. intros Hin. 
+        rewrite Hkey_in_dom in Hin. congruence.
+    Qed.
+
+  End Proofs.
+End GetSpec.
